compiler/backend/proofs/source_to_flatProofScript.sml
@@ -4002,7 +4002,7 @@ val compile_flat_esgc_free = Q.store_thm("compile_flat_esgc_free",
   rw [compile_flat_def, flat_exh_matchTheory.compile_def]
   \\ drule flat_exh_matchProofTheory.compile_decs_esgc_free
   \\ disch_then (qspec_then `init_ctors` mp_tac) \\ rw []
-  \\ drule flat_elimProofTheory.removeFlatProg_esgc_free \\ rw []
+  \\ drule flat_elimProofTheory.remove_flat_prog_esgc_free \\ rw []
   \\ rename1 `compile_decs (compile_decs ds1)`
   \\ irule flat_reorder_matchProofTheory.compile_decs_esgc_free
   \\ irule flat_uncheck_ctorsProofTheory.compile_decs_esgc_free
